update

Assignments/Assignment3.v
@@ -1,205 +1,225 @@
-(** * Assignment 3: COMS E6998 Formal Verification of System Software *)
+(** * Assignment 2: COMS E6998 Formal Verification of System Software *)
 
-(** 
+(**
 
-    - Due 11/20/2020 at 11:59 pm
+    - Due 10/21/2020 at 11:59 pm
     - Replace all the Admitted with your proofs or definitions.
-    - Submit the filled in Assignment3.v via coursework2
+    - Submit the filled in Assignment.v via coursework2
     - Academic Honesty
-      The computer science department has very strict policies. 
+      The computer science department has very strict policies.
       Please read the department [Academic Honesty page](http://www.cs.columbia.edu/education/honesty/).
       You MUST submit original homework written by you and you alone.
-      Do not look at anybody else’s answer. 
+      Do not look at anybody else’s answer.
       Do not show anybody your answer, or leave your answer where somebody else could see it.
       Cases of non-original submission will receive a 0 and will be referred to the Judicial Committee.
 
     1) To compile the assigment, first download the following files
-    
-    _CoqProject
+
     Coq_Lecture1_Basics.v
     Coq_Lecture2_Induction_List.v
-    Coq_Lecture3_Tactics_Logic.v 
-    Coq_Lecture4_Program.v              
-    Assignment3.v
-    
+    Coq_Lecture3_Tactics_Logic.v
+    Assignment2.v
+
     in the same directory.
-    
-    2) Then compile Coq_Lecture4_Program.v by
-    [coqc Coq_Lecture1_Basics Coq_Lecture2_Induction_List Coq_Lecture3_Tactics_Logic Coq_Lecture4_Program]
-    
+
+    2) Then compile Coq_Lecture3_Tactics_Logic.v by
+    [coqc Coq_Lecture1_Basics Coq_Lecture2_Induction_List Coq_Lecture3_Tactics_Logic]
 *)
 
-Require Export Coq_Lecture3_Tactics_Logic Coq_Lecture4_Program.
+Require Import Coq_Lecture3_Tactics_Logic.
 
 (* ################################################################# *)
 (** * Problem 1 *)
 
-(** Prove the following Theorem  *)
-Theorem bool_fn_applied_thrice :
-  forall (f : bool -> bool) (b : bool),
-  f (f (f b)) = f b.
-Proof.
-  (* FILL IN HERE *) Admitted.
-(** [] *)
+Lemma double_negb:
+  forall b, negb (negb b) = b.
+(* FILL IN HERE *) Admitted.
 
 
 (* ################################################################# *)
 (** * Problem 2 *)
 
-(** Prove by induction. *)
+Module Integer.
 
-Theorem filter_exercise : forall (X : Type) (l lf : list X) (test : X -> bool)
-                             (x : X),
-     filter test l = x :: lf ->
-     test x = true.
-Proof.
+  (** In this problem, we will define Integer types together.
+      Let's first define Positive Integers. *)
+
+  Inductive Positive :=
+  | I (* 1 *)
+  | S (p: Positive).
+
+  (** Integher can then be inductively defined using Positive. *)
+  Inductive Integer :=
+  | O (* 0 *)
+  | Pos (p: Positive)
+  | Neg (p: Positive).
+
+  (** Please define the negi function to calculate the negation of an integer *)
+
+  Definition negi (i: Integer): Integer
+  (* REPLACE THIS LINE WITH ":= _your_definition_ ." *). Admitted.
+
+  Example test_negi1: negi O = O.
   (* FILL IN HERE *) Admitted.
-(** [] *)
 
-(* ################################################################# *)
-(** * Problem 3 ~ Problem 6 *)
-(** Old HP Calculators, programming languages like Forth and Postscript,
-    and abstract machines like the Java Virtual Machine all evaluate
-    arithmetic expressions using a _stack_. For instance, the expression
+  Example test_negi2: negi (Pos I) = Neg I.
+  (* FILL IN HERE *) Admitted.
 
-      (2*3)+(3*(4-2))
 
-   would be written as
+  (** Please define the add1 function to add 1 to the given integer *)
+  Definition add1 (i: Integer): Integer
+  (* REPLACE THIS LINE WITH ":= _your_definition_ ." *). Admitted.
 
-      2 3 * 3 4 2 - * +
 
-   and evaluated like this (where we show the program being evaluated
-   on the right and the contents of the stack on the left):
+  Example test_add11: add1 O = Pos I.
+  (* FILL IN HERE *) Admitted.
 
-      [ ]           |    2 3 * 3 4 2 - * +
-      [2]           |    3 * 3 4 2 - * +
-      [3, 2]        |    * 3 4 2 - * +
-      [6]           |    3 4 2 - * +
-      [3, 6]        |    4 2 - * +
-      [4, 3, 6]     |    2 - * +
-      [2, 4, 3, 6]  |    - * +
-      [2, 3, 6]     |    * +
-      [6, 6]        |    +
-      [12]          |
 
-  The goal of the following problems is to write a small compiler that
-  translates [aexp]s into stack machine instructions.
+  Example test_add12: add1 (Neg I) = O.
+  (* FILL IN HERE *) Admitted.
 
-  The instruction set for our stack language will consist of the
-  following instructions:
-     - [SPush n]: Push the number [n] on the stack.
-     - [SLoad x]: Load the identifier [x] from the store and push it
-                  on the stack
-     - [SPlus]:   Pop the two top numbers from the stack, add them, and
-                  push the result onto the stack.
-     - [SMinus]:  Similar, but subtract.
-     - [SMult]:   Similar, but multiply. *)
+  Example test_add13: add1 (Pos I) = Pos (S I).
+  (* FILL IN HERE *) Admitted.
 
-Inductive sinstr : Type :=
-| SPush : nat -> sinstr
-| SLoad : string -> sinstr
-| SPlus : sinstr
-| SMinus : sinstr
-| SMult : sinstr.
+End Integer.
 
 (* ################################################################# *)
 (** * Problem 3 *)
 
-(** Write a function to evaluate programs in the stack language. It
-    should take as input a state, a stack represented as a list of
-    numbers (top stack item is the head of the list), and a program
-    represented as a list of instructions, and it should return the
-    stack after executing the program.  Test your function on the
-    examples below.
+Module NatPlayground3.
 
-    Note that the specification leaves unspecified what to do when
-    encountering an [SPlus], [SMinus], or [SMult] instruction if the
-    stack contains less than two elements. The function should return
-    None for these unspecified cases. But our compiler will never 
-    emit such a malformed program. *)
+  (** In the class, we have defined our own plus and mult for nat. *)
+  Print NatPlayground2.plus.
+  Print NatPlayground2.mult.
 
-(** Execute an instruction **)
-Definition s_execute_instr (st : state) (stack : list nat)
-         (instr : sinstr)
-  : option (list nat)
-(* REPLACE THIS LINE WITH ":= _your_definition_ ." *). Admitted.
-               
-(** Execute a program **)                                           
-Fixpoint s_execute (st : state) (stack : list nat)
-                   (prog : list sinstr)
-  : option (list nat)
-(* REPLACE THIS LINE WITH ":= _your_definition_ ." *). Admitted.
-    
-    
-  
-(*  (* REPLACE THIS LINE WITH ":= _your_definition_ ." *). Admitted.*)
+  (** Let's try to define our own exponential function for nat. *)
+  Fixpoint exp (base power : nat) : nat
+  (* REPLACE THIS LINE WITH ":= _your_definition_ ." *). Admitted.
 
-Example s_execute1 :
-     s_execute { --> 0 } []
-       [SPush 5; SPush 3; SPush 1; SMinus]
-     = Some [2; 5].
-(* FILL IN HERE *) Admitted.
+  Lemma exp_1: forall power, exp 1 power = 1.
+  (* FILL IN HERE *) Admitted.
 
-Example s_execute2 :
-     s_execute { X --> 3 } [3;4]
-       [SPush 4; SLoad X; SMult; SPlus]
-   = Some [15; 4].
-(* FILL IN HERE *) Admitted.
+  Eval compute in (exp 2 4).
+
+End NatPlayground3.
 
 (* ################################################################# *)
 (** * Problem 4 *)
 
-(** Next, write a function that compiles an [aexp] into a stack
-    machine program. The effect of running the program should be the
-    same as pushing the value of the expression on the stack. *)
+Module NatPlayground4.
 
-Fixpoint s_compile (e : aexp) : list sinstr
-(* REPLACE THIS LINE WITH ":= _your_definition_ ." *). Admitted.
+  (** Let's prove some properties of plus and mult  *)
+  Theorem plus_assoc : forall m n t : nat,
+      m + (n + t) = m + n + t.
+  (* FILL IN HERE *) Admitted.
 
-(** After you've defined [s_compile], prove the following to test
-    that it works. *)
+  (** Hint use plus_assoc and plus_comm *)
+  Theorem plus_comm' : forall m n t : nat,
+      m + n + t = m + t + n.
+  (* FILL IN HERE *) Admitted.
 
-Local Open Scope aexp_scope.
+  (** Hint use plus_assoc and plus_comm' *)
+  Theorem mult_plus_distr : forall m n t : nat,
+      m * (n + t) = m * n + m * t.
+  (* FILL IN HERE *) Admitted.
 
-Example s_compile1 :
-  s_compile (X .- (2 .* Y))
-  = [SLoad X; SPush 2; SLoad Y; SMult; SMinus].
-(* FILL IN HERE *) Admitted.
-(** [] *)
+End NatPlayground4.
+
 
 (* ################################################################# *)
 (** * Problem 5 *)
 
-(** Prove the following property for s_execute *)
-Theorem s_execute_mono : forall (l1 l2: list sinstr) (sk sk': list nat) (st : state),
-  s_execute st sk l1 = Some sk' ->
-  s_execute st sk (l1 ++ l2) = s_execute st sk' l2.
+(** Prove the following properties over beq_nat *)
+Print beq_nat.
+
+Lemma beq_nat_eq:
+  forall n m,
+    beq_nat n m = true ->
+    n = m.
+(* FILL IN HERE *) Admitted.
+
+Lemma beq_nat_eq':
+  forall n m,
+    n = m
+    -> beq_nat n m = true.
+(* FILL IN HERE *) Admitted.
+
+(** Hint: recall the Lecure for logic *)
+Theorem zero_not_one : ~(0 = 1).
 Proof.
-  (* FILL IN HERE *) Admitted.
-(** [] *)    
+  intros contra. inversion contra.
+Qed.
+
+Lemma beq_nat_neq:
+  forall n m,
+    beq_nat n m = false ->
+    n <> m.
+(* FILL IN HERE *) Admitted.
+
+(** Hint use ex_falso_quodlibet *)
+Lemma beq_nat_neq':
+  forall n m,
+    n <> m
+    -> beq_nat n m = false.
+(* FILL IN HERE *) Admitted.
+
 
 (* ################################################################# *)
 (** * Problem 6 *)
-    
-(** Now we'll prove the correctness of the compiler implemented in the
-    previous exercise.  Remember that the specification left
-    unspecified what to do when encountering an [SPlus], [SMinus], or
-    [SMult] instruction if the stack contains less than two
-    elements.  (In order to make your correctness proof easier you
-    might find it helpful to go back and change your implementation!)
 
-    Prove the following theorem.  You will need to start by stating a
-    more general lemma to get a usable induction hypothesis; the main
-    theorem will then be a simple corollary of this lemma. *)
+(** *** Bags via Lists *)
 
-Theorem s_compile_correct' : forall (e : aexp) (sk: list nat) (st : state),
-  s_execute st sk (s_compile e) = Some (aeval st e :: sk).
-Proof.
-  (* FILL IN HERE *) Admitted.
-(** [] *)
+(** A [bag] (or [multiset]) is like a set, except that each element
+    can appear multiple times rather than just once.  One possible
+    implementation is to represent a bag of numbers as a list. *)
 
-Theorem s_compile_correct : forall (st : state) (e : aexp),
-  s_execute st [] (s_compile e) = Some [ aeval st e ].
-Proof.
-  (* FILL IN HERE *) Admitted.
+Definition bag := list nat.
+
+(** Complete the following definitions for the functions
+    [count], [sum], [add], and [member] for bags. *)
+
+Fixpoint count (v:nat) (s:bag) : nat
+(* REPLACE THIS LINE WITH ":= _your_definition_ ." *). Admitted.
+
+(** All these proofs can be done just by [reflexivity]. *)
+Example test_count1:              count 1 [1;2;3;1;4;1] = 3.
+ (* FILL IN HERE *) Admitted.
+Example test_count2:              count 6 [1;2;3;1;4;1] = 0.
+simpl.
+ (* FILL IN HERE *) Admitted.
+
+(** Multiset [sum] is similar to set [union]: [sum a b] contains all
+    the elements of [a] and of [b].  (Mathematicians usually define
+    [union] on multisets a little bit differently -- using max instead
+    of sum -- which is why we don't use that name for this operation.)
+    For [sum] we're giving you a header that does not give explicit
+    names to the arguments.  Moreover, it uses the keyword
+    [Definition] instead of [Fixpoint], so even if you had names for
+    the arguments, you wouldn't be able to process them recursively.
+    The point of stating the question this way is to encourage you to
+    think about whether [sum] can be implemented in another way --
+    perhaps by using functions that have already been defined.  *)
+
+Definition sum : bag -> bag -> bag
+  (* REPLACE THIS LINE WITH ":= _your_definition_ ." *). Admitted.
+
+Example test_sum1:              count 1 (sum [1;2;3] [1;4;1]) = 3.
+ (* FILL IN HERE *) Admitted.
+
+Definition add (v:nat) (s:bag) : bag
+  (* REPLACE THIS LINE WITH ":= _your_definition_ ." *). Admitted.
+
+Example test_add1:                count 1 (add 1 [1;4;1]) = 3.
+ (* FILL IN HERE *) Admitted.
+Example test_add2:                count 5 (add 1 [1;4;1]) = 0.
+ (* FILL IN HERE *) Admitted.
+
+Definition member (v:nat) (s:bag) : bool
+  (* REPLACE THIS LINE WITH ":= _your_definition_ ." *). Admitted.
+
+Example test_member1:             member 1 [1;4;1] = true.
+ (* FILL IN HERE *) Admitted.
+
+Example test_member2:             member 2 [1;4;1] = false.
+(* FILL IN HERE *) Admitted.
 (** [] *)
