Assignments/Assignment4.v
@@ -1,10 +1,10 @@
-(** * Assignment 4: COMS E6998 Formal Verification of System Software *)
+(** * Assignment 3: COMS E6998 Formal Verification of System Software *)
 
 (** 
 
-    - Due 11/27/2020 at 11:59 pm
+    - Due 11/20/2020 at 11:59 pm
     - Replace all the Admitted with your proofs or definitions.
-    - Submit the filled in Assignment4.v via coursework2
+    - Submit the filled in Assignment3.v via coursework2
     - Academic Honesty
       The computer science department has very strict policies. 
       Please read the department [Academic Honesty page](http://www.cs.columbia.edu/education/honesty/).
@@ -15,232 +15,191 @@
 
     1) To compile the assigment, first download the following files
     
-    _CoqProject 
+    _CoqProject
+    Coq_Lecture1_Basics.v
+    Coq_Lecture2_Induction_List.v
+    Coq_Lecture3_Tactics_Logic.v 
     Coq_Lecture4_Program.v              
-    Assignment4.v
+    Assignment3.v
     
     in the same directory.
     
     2) Then compile Coq_Lecture4_Program.v by
-    [coqc Coq_Lecture4_Program]
-
+    [coqc Coq_Lecture1_Basics Coq_Lecture2_Induction_List Coq_Lecture3_Tactics_Logic Coq_Lecture4_Program]
     
-    [make]
 *)
 
-Require Import Coq.Bool.Bool.
-Require Import Coq.Arith.Arith.
-Require Import Coq.Arith.EqNat.
-Require Import Coq.omega.Omega.
-Require Import Coq.Lists.List.
-Import ListNotations.
-
-Require Export Coq_Lecture4_Program.
-
-(** * Problem 1 ~ Problem 6 *)
-(** Imperative languages like C and Java often include a [break] or
-    similar statement for interrupting the execution of loops. In this
-    assignment we consider how to add [break] to Imp.  First, we need to
-    enrich the language of commands with an additional case. *)
-
-Inductive com : Type :=
-  | CSkip : com
-  | CBreak : com               (* <-- new *)
-  | CAss : string -> aexp -> com
-  | CSeq : com -> com -> com
-  | CIf : bexp -> com -> com -> com
-  | CWhile : bexp -> com -> com.
-
-Notation "'SKIP'" :=
-  CSkip.
-Notation "'BREAK'" :=
-  CBreak.
-Notation "x '::=' a" :=
-  (CAss x a) (at level 60).
-Notation "c1 ;; c2" :=
-  (CSeq c1 c2) (at level 80, right associativity).
-Notation "'WHILE' b 'DO' c 'END'" :=
-  (CWhile b c) (at level 80, right associativity).
-Notation "'IFB' c1 'THEN' c2 'ELSE' c3 'FI'" :=
-  (CIf c1 c2 c3) (at level 80, right associativity).
-
-(** Next, we need to define the behavior of [BREAK].  Informally,
-    whenever [BREAK] is executed in a sequence of commands, it stops
-    the execution of that sequence and signals that the innermost
-    enclosing loop should terminate.  (If there aren't any
-    enclosing loops, then the whole program simply terminates.)  The
-    final state should be the same as the one in which the [BREAK]
-    statement was executed.
-
-    One important point is what to do when there are multiple loops
-    enclosing a given [BREAK]. In those cases, [BREAK] should only
-    terminate the _innermost_ loop. Thus, after executing the
-    following...
-
-       X ::= 0;;
-       Y ::= 1;;
-       WHILE 0 <> Y DO
-         WHILE TRUE DO
-           BREAK
-         END;;
-         X ::= 1;;
-         Y ::= Y .- 1
-       END
-
-    ... the value of [X] should be [1], and not [0].
-
-    One way of expressing this behavior is to add another parameter to
-    the evaluation relation that specifies whether evaluation of a
-    command executes a [BREAK] statement: *)
-
-Inductive result : Type :=
-  | SContinue : result
-  | SBreak : result.
-
-Reserved Notation "c1 '/' st '\\' s '/' st'"
-                  (at level 40, st, s at level 39).
-
-(** Intuitively, [c / st \\ s / st'] means that, if [c] is started in
-    state [st], then it terminates in state [st'] and either signals
-    that the innermost surrounding loop (or the whole program) should
-    exit immediately ([s = SBreak]) or that execution should continue
-    normally ([s = SContinue]).
-
-    The definition of the "[c / st \\ s / st']" relation is very
-    similar to the one we gave above for the regular evaluation
-    relation ([c / st \\ st']) -- we just need to handle the
-    termination signals appropriately:
-
-    - If the command is [SKIP], then the state doesn't change and
-      execution of any enclosing loop can continue normally.
-
-    - If the command is [BREAK], the state stays unchanged but we
-      signal a [SBreak].
-
-    - If the command is an assignment, then we update the binding for
-      that variable in the state accordingly and signal that execution
-      can continue normally.
-
-    - If the command is of the form [IFB b THEN c1 ELSE c2 FI], then
-      the state is updated as in the original semantics of Imp, except
-      that we also propagate the signal from the execution of
-      whichever branch was taken.
-
-    - If the command is a sequence [c1 ;; c2], we first execute
-      [c1].  If this yields a [SBreak], we skip the execution of [c2]
-      and propagate the [SBreak] signal to the surrounding context;
-      the resulting state is the same as the one obtained by
-      executing [c1] alone. Otherwise, we execute [c2] on the state
-      obtained after executing [c1], and propagate the signal
-      generated there.
-
-    - Finally, for a loop of the form [WHILE b DO c END], the
-      semantics is almost the same as before. The only difference is
-      that, when [b] evaluates to true, we execute [c] and check the
-      signal that it raises.  If that signal is [SContinue], then the
-      execution proceeds as in the original semantics. Otherwise, we
-      stop the execution of the loop, and the resulting state is the
-      same as the one resulting from the execution of the current
-      iteration.  In either case, since [BREAK] only terminates the
-      innermost loop, [WHILE] signals [SContinue]. *)
+Require Export Coq_Lecture3_Tactics_Logic Coq_Lecture4_Program.
 
 (* ################################################################# *)
 (** * Problem 1 *)
 
-(** Based on the above description, complete the definition of the
-    [ceval] relation. *)
-
-Inductive ceval : com -> state -> result -> state -> Prop :=
-  | E_Skip : forall st,
-      CSkip / st \\ SContinue / st
-  (* FILL IN HERE *)
-
-  where "c1 '/' st '\\' s '/' st'" := (ceval c1 st s st').
-
-Local Open Scope aexp_scope.
-Local Open Scope bexp_scope.
-
-Definition example: com :=
-  X ::= 0;;
-  Y ::= 1;;
-  WHILE !(0 =? Y) DO
-    WHILE true DO
-      BREAK
-    END;;
-    X ::= 1;;
-    Y ::= Y .- 1
-  END.
-
-Ltac inversion_program st :=
-  match goal with
-  | [Htf: true = false |- _] => inversion Htf
-  | [Hft: false = true |- _] => inversion Hft
-  | [Hst0: _ / ?st0 \\ _ / _  |- _ ] =>
-    match st0 with
-    | context[st] => (* context[st] means that the term contains st*)
-      inversion Hst0; subst; simpl in *; clear Hst0
-    end
-  end.
-
-Theorem ceval_example:
-  forall st st',
-    example / st \\ SContinue / st' ->
-    st' X = 1 /\ st' Y = 0.
+(** Prove the following Theorem  *)
+Theorem bool_fn_applied_thrice :
+  forall (f : bool -> bool) (b : bool),
+  f (f (f b)) = f b.
 Proof.
-  (* Please fix the following proof if it is broken by your definition.
-  intros.
-  repeat inversion_program st.
-  rewrite t_update_eq.
-  rewrite t_update_neq.
-  - rewrite t_update_eq. split; reflexivity.
-  - intro HF; inversion HF. 
-Qed.
-*)
-Admitted.
+  (* FILL IN HERE *) Admitted.
+(** [] *)
+
 
 (* ################################################################# *)
 (** * Problem 2 *)
-Theorem break_ignore : forall c st st' s,
-     (BREAK;; c) / st \\ s / st' ->
-     st = st'.
+
+(** Prove by induction. *)
+
+Theorem filter_exercise : forall (X : Type) (l lf : list X) (test : X -> bool)
+                             (x : X),
+     filter test l = x :: lf ->
+     test x = true.
 Proof.
   (* FILL IN HERE *) Admitted.
+(** [] *)
+
+(* ################################################################# *)
+(** * Problem 3 ~ Problem 6 *)
+(** Old HP Calculators, programming languages like Forth and Postscript,
+    and abstract machines like the Java Virtual Machine all evaluate
+    arithmetic expressions using a _stack_. For instance, the expression
+
+      (2*3)+(3*(4-2))
+
+   would be written as
+
+      2 3 * 3 4 2 - * +
+
+   and evaluated like this (where we show the program being evaluated
+   on the right and the contents of the stack on the left):
+
+      [ ]           |    2 3 * 3 4 2 - * +
+      [2]           |    3 * 3 4 2 - * +
+      [3, 2]        |    * 3 4 2 - * +
+      [6]           |    3 4 2 - * +
+      [3, 6]        |    4 2 - * +
+      [4, 3, 6]     |    2 - * +
+      [2, 4, 3, 6]  |    - * +
+      [2, 3, 6]     |    * +
+      [6, 6]        |    +
+      [12]          |
+
+  The goal of the following problems is to write a small compiler that
+  translates [aexp]s into stack machine instructions.
+
+  The instruction set for our stack language will consist of the
+  following instructions:
+     - [SPush n]: Push the number [n] on the stack.
+     - [SLoad x]: Load the identifier [x] from the store and push it
+                  on the stack
+     - [SPlus]:   Pop the two top numbers from the stack, add them, and
+                  push the result onto the stack.
+     - [SMinus]:  Similar, but subtract.
+     - [SMult]:   Similar, but multiply. *)
+
+Inductive sinstr : Type :=
+| SPush : nat -> sinstr
+| SLoad : string -> sinstr
+| SPlus : sinstr
+| SMinus : sinstr
+| SMult : sinstr.
 
 (* ################################################################# *)
 (** * Problem 3 *)
-Theorem while_continue : forall b c st st' s,
-  (WHILE b DO c END) / st \\ s / st' ->
-  s = SContinue.
-Proof.
-  (* FILL IN HERE *) Admitted.
 
-(* ################################################################# *)
-(** * Problem 4 *)
-Theorem while_stops_on_break : forall b c st st',
-  beval st b = true ->
-  c / st \\ SBreak / st' ->
-  (WHILE b DO c END) / st \\ SContinue / st'.
-Proof.
-  (* FILL IN HERE *) Admitted.
+(** Write a function to evaluate programs in the stack language. It
+    should take as input a state, a stack represented as a list of
+    numbers (top stack item is the head of the list), and a program
+    represented as a list of instructions, and it should return the
+    stack after executing the program.  Test your function on the
+    examples below.
 
-(* ################################################################# *)
-(** * Problem 5 *)
-(** Hint: use induction over He **)
-Theorem while_break_true :
-  forall p b c st st' 
-         (Heq: p = (WHILE b DO c END))
-         (He: p / st \\ SContinue / st')
-         (Heval: beval st' b = true),
-    exists st'', c / st'' \\ SBreak / st'.
-Proof.
+    Note that the specification leaves unspecified what to do when
+    encountering an [SPlus], [SMinus], or [SMult] instruction if the
+    stack contains less than two elements. The function should return
+    None for these unspecified cases. But our compiler will never 
+    emit such a malformed program. *)
+
+(** Execute an instruction **)
+Definition s_execute_instr (st : state) (stack : list nat)
+         (instr : sinstr)
+  : option (list nat)
+(* REPLACE THIS LINE WITH ":= _your_definition_ ." *). Admitted.
+               
+(** Execute a program **)                                           
+Fixpoint s_execute (st : state) (stack : list nat)
+                   (prog : list sinstr)
+  : option (list nat)
+(* REPLACE THIS LINE WITH ":= _your_definition_ ." *). Admitted.
+    
+    
+  
+(*  (* REPLACE THIS LINE WITH ":= _your_definition_ ." *). Admitted.*)
+
+Example s_execute1 :
+     s_execute { --> 0 } []
+       [SPush 5; SPush 3; SPush 1; SMinus]
+     = Some [2; 5].
+(* FILL IN HERE *) Admitted.
+
+Example s_execute2 :
+     s_execute { X --> 3 } [3;4]
+       [SPush 4; SLoad X; SMult; SPlus]
+   = Some [15; 4].
 (* FILL IN HERE *) Admitted.
 
 (* ################################################################# *)
-(** * Problem 6 *)
-(** Hint: refer to the deterministic for the original com taught in class **)
-Theorem ceval_deterministic: forall (c:com) st st1 st2 s1 s2,
-     c / st \\ s1 / st1  ->
-     c / st \\ s2 / st2 ->
-     st1 = st2 /\ s1 = s2.
+(** * Problem 4 *)
+
+(** Next, write a function that compiles an [aexp] into a stack
+    machine program. The effect of running the program should be the
+    same as pushing the value of the expression on the stack. *)
+
+Fixpoint s_compile (e : aexp) : list sinstr
+(* REPLACE THIS LINE WITH ":= _your_definition_ ." *). Admitted.
+
+(** After you've defined [s_compile], prove the following to test
+    that it works. *)
+
+Local Open Scope aexp_scope.
+
+Example s_compile1 :
+  s_compile (X .- (2 .* Y))
+  = [SLoad X; SPush 2; SLoad Y; SMult; SMinus].
+(* FILL IN HERE *) Admitted.
+(** [] *)
+
+(* ################################################################# *)
+(** * Problem 5 *)
+
+(** Prove the following property for s_execute *)
+Theorem s_execute_mono : forall (l1 l2: list sinstr) (sk sk': list nat) (st : state),
+  s_execute st sk l1 = Some sk' ->
+  s_execute st sk (l1 ++ l2) = s_execute st sk' l2.
 Proof.
   (* FILL IN HERE *) Admitted.
+(** [] *)    
+
+(* ################################################################# *)
+(** * Problem 6 *)
+    
+(** Now we'll prove the correctness of the compiler implemented in the
+    previous exercise.  Remember that the specification left
+    unspecified what to do when encountering an [SPlus], [SMinus], or
+    [SMult] instruction if the stack contains less than two
+    elements.  (In order to make your correctness proof easier you
+    might find it helpful to go back and change your implementation!)
+
+    Prove the following theorem.  You will need to start by stating a
+    more general lemma to get a usable induction hypothesis; the main
+    theorem will then be a simple corollary of this lemma. *)
+
+Theorem s_compile_correct' : forall (e : aexp) (sk: list nat) (st : state),
+  s_execute st sk (s_compile e) = Some (aeval st e :: sk).
+Proof.
+  (* FILL IN HERE *) Admitted.
+(** [] *)
+
+Theorem s_compile_correct : forall (st : state) (e : aexp),
+  s_execute st [] (s_compile e) = Some [ aeval st e ].
+Proof.
+  (* FILL IN HERE *) Admitted.
+(** [] *)
