Assignments/Assignment5.v
@@ -1,30 +1,31 @@
-(** * Assignment 5: COMS E6998 Formal Verification of System Software *)
+(** * Assignment 4: COMS E6998 Formal Verification of System Software *)
 
-(**
+(** 
 
-    - Due 12/21/2020 at 11:59 pm
+    - Due 11/27/2020 at 11:59 pm
     - Replace all the Admitted with your proofs or definitions.
-    - Submit the filled in Assignment5.v via coursework2
+    - Submit the filled in Assignment4.v via coursework2
     - Academic Honesty
-      The computer science department has very strict policies.
+      The computer science department has very strict policies. 
       Please read the department [Academic Honesty page](http://www.cs.columbia.edu/education/honesty/).
       You MUST submit original homework written by you and you alone.
-      Do not look at anybody else’s answer.
+      Do not look at anybody else’s answer. 
       Do not show anybody your answer, or leave your answer where somebody else could see it.
       Cases of non-original submission will receive a 0 and will be referred to the Judicial Committee.
 
     1) To compile the assigment, first download the following files
-
-    Coq_Lecture4_Program.v
-    Coq_Lecture5_Hoare.v
-    Assignment5.v
-
+    
+    _CoqProject 
+    Coq_Lecture4_Program.v              
+    Assignment4.v
+    
     in the same directory.
+    
+    2) Then compile Coq_Lecture4_Program.v by
+    [coqc Coq_Lecture4_Program]
 
-    2) Then compile Coq_Lecture4_Program.v and Coq_Lecture5_Hoare.v by
-    [coqc Coq_Lecture4_Program.v]
-    [coqc Coq_Lecture5_Hoare.v]
-
+    
+    [make]
 *)
 
 Require Import Coq.Bool.Bool.
@@ -34,342 +35,212 @@ Require Import Coq.omega.Omega.
 Require Import Coq.Lists.List.
 Import ListNotations.
 
-Require Import Coq_Lecture4_Program.
-Require Export Coq_Lecture5_Hoare.
+Require Export Coq_Lecture4_Program.
+
+(** * Problem 1 ~ Problem 6 *)
+(** Imperative languages like C and Java often include a [break] or
+    similar statement for interrupting the execution of loops. In this
+    assignment we consider how to add [break] to Imp.  First, we need to
+    enrich the language of commands with an additional case. *)
+
+Inductive com : Type :=
+  | CSkip : com
+  | CBreak : com               (* <-- new *)
+  | CAss : string -> aexp -> com
+  | CSeq : com -> com -> com
+  | CIf : bexp -> com -> com -> com
+  | CWhile : bexp -> com -> com.
+
+Notation "'SKIP'" :=
+  CSkip.
+Notation "'BREAK'" :=
+  CBreak.
+Notation "x '::=' a" :=
+  (CAss x a) (at level 60).
+Notation "c1 ;; c2" :=
+  (CSeq c1 c2) (at level 80, right associativity).
+Notation "'WHILE' b 'DO' c 'END'" :=
+  (CWhile b c) (at level 80, right associativity).
+Notation "'IFB' c1 'THEN' c2 'ELSE' c3 'FI'" :=
+  (CIf c1 c2 c3) (at level 80, right associativity).
+
+(** Next, we need to define the behavior of [BREAK].  Informally,
+    whenever [BREAK] is executed in a sequence of commands, it stops
+    the execution of that sequence and signals that the innermost
+    enclosing loop should terminate.  (If there aren't any
+    enclosing loops, then the whole program simply terminates.)  The
+    final state should be the same as the one in which the [BREAK]
+    statement was executed.
+
+    One important point is what to do when there are multiple loops
+    enclosing a given [BREAK]. In those cases, [BREAK] should only
+    terminate the _innermost_ loop. Thus, after executing the
+    following...
+
+       X ::= 0;;
+       Y ::= 1;;
+       WHILE 0 <> Y DO
+         WHILE TRUE DO
+           BREAK
+         END;;
+         X ::= 1;;
+         Y ::= Y .- 1
+       END
+
+    ... the value of [X] should be [1], and not [0].
+
+    One way of expressing this behavior is to add another parameter to
+    the evaluation relation that specifies whether evaluation of a
+    command executes a [BREAK] statement: *)
+
+Inductive result : Type :=
+  | SContinue : result
+  | SBreak : result.
+
+Reserved Notation "c1 '/' st '\\' s '/' st'"
+                  (at level 40, st, s at level 39).
+
+(** Intuitively, [c / st \\ s / st'] means that, if [c] is started in
+    state [st], then it terminates in state [st'] and either signals
+    that the innermost surrounding loop (or the whole program) should
+    exit immediately ([s = SBreak]) or that execution should continue
+    normally ([s = SContinue]).
+
+    The definition of the "[c / st \\ s / st']" relation is very
+    similar to the one we gave above for the regular evaluation
+    relation ([c / st \\ st']) -- we just need to handle the
+    termination signals appropriately:
+
+    - If the command is [SKIP], then the state doesn't change and
+      execution of any enclosing loop can continue normally.
+
+    - If the command is [BREAK], the state stays unchanged but we
+      signal a [SBreak].
+
+    - If the command is an assignment, then we update the binding for
+      that variable in the state accordingly and signal that execution
+      can continue normally.
+
+    - If the command is of the form [IFB b THEN c1 ELSE c2 FI], then
+      the state is updated as in the original semantics of Imp, except
+      that we also propagate the signal from the execution of
+      whichever branch was taken.
+
+    - If the command is a sequence [c1 ;; c2], we first execute
+      [c1].  If this yields a [SBreak], we skip the execution of [c2]
+      and propagate the [SBreak] signal to the surrounding context;
+      the resulting state is the same as the one obtained by
+      executing [c1] alone. Otherwise, we execute [c2] on the state
+      obtained after executing [c1], and propagate the signal
+      generated there.
+
+    - Finally, for a loop of the form [WHILE b DO c END], the
+      semantics is almost the same as before. The only difference is
+      that, when [b] evaluates to true, we execute [c] and check the
+      signal that it raises.  If that signal is [SContinue], then the
+      execution proceeds as in the original semantics. Otherwise, we
+      stop the execution of the loop, and the resulting state is the
+      same as the one resulting from the execution of the current
+      iteration.  In either case, since [BREAK] only terminates the
+      innermost loop, [WHILE] signals [SContinue]. *)
+
+(* ################################################################# *)
+(** * Problem 1 *)
+
+(** Based on the above description, complete the definition of the
+    [ceval] relation. *)
+
+Inductive ceval : com -> state -> result -> state -> Prop :=
+  | E_Skip : forall st,
+      CSkip / st \\ SContinue / st
+  (* FILL IN HERE *)
+
+  where "c1 '/' st '\\' s '/' st'" := (ceval c1 st s st').
 
 Local Open Scope aexp_scope.
 Local Open Scope bexp_scope.
 
-(** As we discussed in the last lecture, some decorations inof dcom are redundant.
-    In this assignment, we will design a new dcom which only contains the pre- and post-conditions,
-    plus the loop invariants *)
+Definition example: com :=
+  X ::= 0;;
+  Y ::= 1;;
+  WHILE !(0 =? Y) DO
+    WHILE true DO
+      BREAK
+    END;;
+    X ::= 1;;
+    Y ::= Y .- 1
+  END.
 
-Inductive dcom : Type :=
-| DCSkip
-| DCSeq (d1 d2:  dcom)
-| DCAsgn (X: string) (e: aexp)
-| DCIf (b: bexp) (d1: dcom) (d2: dcom)
-| DCWhile (b: bexp) (inv: Assertion) (body: dcom).
-
-Inductive decorated : Type :=
-  | Decorated : Assertion -> dcom -> Assertion -> decorated.
-
-Delimit Scope decorated_scope with decorated.
-
-Notation "'SKIP'" := DCSkip.
-Notation "l '::=' a"
-  := (DCAsgn l a)
-       (at level 60, a at next level) : decorated_scope.
-Notation "'WHILE' b [[ INV ]] 'DO'  d 'END'"
-  := (DCWhile b INV d)
-       (at level 80, right associativity) : decorated_scope.
-Notation "'IFB' b 'THEN' d 'ELSE' d' 'FI'"
-  := (DCIf b d d')
-       (at level 80, right associativity) : decorated_scope.
-Notation " d ;; d' "
-  := (DCSeq d d')
-       (at level 80, right associativity) : decorated_scope.
-Notation "[[ P ]] d [[ Q ]]"
-  := (Decorated P d Q) (at level 90, d at next level) : decorated_scope.
-
-Open Scope decorated_scope.
-
-Example dec_while : decorated :=
-  [[ fun st => True ]]
-  WHILE !(X =? 0)
-  [[ fun _ => True ]]
-  DO
-    X ::= X .- 1
-  END
-  [[ fun st => st X = 0 ]].
-
-(* ################################################################# *)
-(** * Problem 1 *)
-(** It is easy to go from a [dcom] to a [com] by erasing all
-    annotations. *)
-Fixpoint extract (d:dcom) : com
-(* REPLACE THIS LINE WITH ":= _your_definition_ ." *). Admitted.
-
-Definition extract_dec (dec : decorated) : com :=
-  match dec with
-  | Decorated _ d _ => extract d
+Ltac inversion_program st :=
+  match goal with
+  | [Htf: true = false |- _] => inversion Htf
+  | [Hft: false = true |- _] => inversion Hft
+  | [Hst0: _ / ?st0 \\ _ / _  |- _ ] =>
+    match st0 with
+    | context[st] => (* context[st] means that the term contains st*)
+      inversion Hst0; subst; simpl in *; clear Hst0
+    end
   end.
 
-Local Open Scope com_scope.
-
-Example extract_correct:
-  extract_dec dec_while =
-  WHILE !(X =? 0)
-  DO
-    X ::= X .- 1
-  END.
-Proof. (* FILL IN HERE *) Admitted.
+Theorem ceval_example:
+  forall st st',
+    example / st \\ SContinue / st' ->
+    st' X = 1 /\ st' Y = 0.
+Proof.
+  (* Please fix the following proof if it is broken by your definition.
+  intros.
+  repeat inversion_program st.
+  rewrite t_update_eq.
+  rewrite t_update_neq.
+  - rewrite t_update_eq. split; reflexivity.
+  - intro HF; inversion HF. 
+Qed.
+*)
+Admitted.
 
 (* ################################################################# *)
 (** * Problem 2 *)
-(** It is straightforward to extract the precondition and
-    postcondition from a decorated program. *)
-
-Definition pre_dec (dec : decorated) : Assertion
-(* REPLACE THIS LINE WITH ":= _your_definition_ ." *). Admitted.
-
-Definition post_dec (dec : decorated) : Assertion
-(* REPLACE THIS LINE WITH ":= _your_definition_ ." *). Admitted.
-
-(** We can express what it means for a decorated program to be
-    correct as follows: *)
-Definition dec_correct (dec : decorated): Prop
-(* REPLACE THIS LINE WITH ":= _your_definition_ ." *). Admitted.
-
-Example dec_correct_correct:
-  dec_correct dec_while =
-  {{ fun st => True }}
-  WHILE !(X =? 0)
-  DO
-    X ::= X .- 1
-  END
-  {{ fun st => st X = 0 }}.
-Proof. (* FILL IN HERE *) Admitted.
+Theorem break_ignore : forall c st st' s,
+     (BREAK;; c) / st \\ s / st' ->
+     st = st'.
+Proof.
+  (* FILL IN HERE *) Admitted.
 
 (* ################################################################# *)
 (** * Problem 3 *)
-(** To check whether this Hoare triple is _valid_, we need a way to
-    extract the "proof obligations" or the verification conditions
-    from a decorated program. The function [VC] takes a [dcom] [d] together
-    with a postcondition [Q] and returns a pair of assertions (wp, sd).
-    [wp] stands for a weak precondition, while [sd] stands for the
-    side conditions that have to hold. Note that this wp is not the
-    weakest precondition and sd is used to show that the given loop invariants
-    satisfy the required conditions*)
-
-Definition assert_implies (P Q : Assertion) : Assertion :=
-  fun st =>  P st -> Q st.
-Definition assert_and (P Q : Assertion) : Assertion :=
-  fun st =>  P st /\ Q st.
-Definition assert_not (P : Assertion) : Assertion :=
-  fun st =>  ~ P st.
-Definition ATrue : Assertion :=
-  fun st => True.
-
-Notation "P ->> Q" := (assert_implies P Q) (at level 80).
-Notation "P //\ Q" := (assert_and P Q) (at level 70).
-Notation "~~ P" := (assert_not P) (at level 60).
-
-Fixpoint VC (d:dcom) (Q : Assertion) : Assertion * Assertion :=
-  match d with
-    (* Skip: wp is Q and no side conditions *)
-  | DCSkip => (Q, ATrue)
-    (* Seq: wp is calculated using wp2 of d2.
-       sd is the conjunction of sd1 and sd2 since the validity
-       of loop invariants are independent
-       *)
-  | DCSeq d1 d2 =>
-    match VC d2 Q with
-    | (wp2, sd2) =>
-      match VC d1 wp2 with
-      | (wp1, sd1) =>
-        (wp1, sd1 //\ sd2)
-      end
-    end
-  | DCAsgn X a => (Q [a // X], ATrue)
-
-  (* If: again the validity of loop invariants in different
-     branches are independent *)
-  | DCIf b d1 d2 =>
-    match VC d1 Q, VC d2 Q with
-    | (wp1, sd1), (wp2, sd2) =>
-      ((bassn b ->> wp1)
-         //\ (~~(bassn b) ->> wp2),
-       (sd1 //\ sd2))
-    end
-
-  (* While: wp is the loop invariants.
-     sd checks
-     1) inv & b implies the wp of the loop body;
-     2) sd of the loop body holds;
-     3) inv & ~b implies the post condition *)
-  | DCWhile b INV d =>
-    (INV,
-     match VC d INV with
-     | (wp, sd) =>
-       (INV //\ bassn b ->> wp)
-         //\ sd
-         //\ (INV //\ ~~(bassn b) ->> Q)
-     end)
-end.
-
-(** The verification condition for the decorated program is that
-    1) the precondition implies wp;
-    2) sd always hold *)
-Definition VC_dec (dec : decorated) : Prop :=
-  match dec with
-  | Decorated P d Q =>
-    match VC d Q with
-    | (wp, sd) =>
-      forall st, (P st -> wp st) /\ sd st
-    end
-  end.
-
-(** And now the key theorem, stating that [verification_conditions]
-    does its job correctly.  Not surprisingly, we need to use each of
-    the Hoare Logic rules at some point in the proof. *)
-Theorem verification_correct : forall d,
-  VC_dec d -> dec_correct d.
+Theorem while_continue : forall b c st st' s,
+  (WHILE b DO c END) / st \\ s / st' ->
+  s = SContinue.
 Proof.
-  destruct d as [P d Q].
-  generalize dependent Q.
-  generalize dependent P.
-  (* FILL IN HERE, HINT: use induction *) Admitted.
+  (* FILL IN HERE *) Admitted.
 
 (* ################################################################# *)
 (** * Problem 4 *)
-(** Now that all the pieces are in place, we can build tactics to verify programs. *)
-
-Ltac my_simpl :=
-(* REPLACE THIS LINE WITH ":= _your_definition_ ." *) idtac.
-
-Ltac verify :=
-(* REPLACE THIS LINE WITH ":= _your_definition_ ." *) idtac.
+Theorem while_stops_on_break : forall b c st st',
+  beval st b = true ->
+  c / st \\ SBreak / st' ->
+  (WHILE b DO c END) / st \\ SContinue / st'.
+Proof.
+  (* FILL IN HERE *) Admitted.
 
 (* ################################################################# *)
 (** * Problem 5 *)
-(** In this program, we use the automation developed above to verify
-    formal decorated programs. *)
+(** Hint: use induction over He **)
+Theorem while_break_true :
+  forall p b c st st' 
+         (Heq: p = (WHILE b DO c END))
+         (He: p / st \\ SContinue / st')
+         (Heval: beval st' b = true),
+    exists st'', c / st'' \\ SBreak / st'.
+Proof.
+(* FILL IN HERE *) Admitted.
 
-Theorem dec_while_correct :
-  dec_correct dec_while.
-(* FILL IN HERE using verify tactic *) Admitted.
-
-Open Scope decorated_scope.
-
-Example subtract_slowly_dec (m:nat) (p:nat) : decorated :=
-  [[ fun st => st X = m /\ st Z = p ]]
-  WHILE ! (X =? 0)
-  [[ fun st => st Z - st X = p - m ]]
-  DO
-     Z ::= Z .- 1;;
-     X ::= X .- 1
-  END
-  [[ fun st => st Z = p - m ]].
-
-Theorem subtract_slowly_dec_correct : forall m p,
-    dec_correct (subtract_slowly_dec m p).
-(* FILL IN HERE using verify tactic *) Admitted.
-
-
-(* ----------------------------------------------------------------- *)
-(** *** Swapping Using Addition and Subtraction *)
-Open Scope com_scope.
-
-Definition swap : com :=
-  X ::= X .+ Y;;
-  Y ::= X .- Y;;
-  X ::= X .- Y.
-
-Open Scope decorated_scope.
-
-Definition swap_dec m n : decorated :=
-  [[ fun st => st X = m /\ st Y = n ]]
-  X ::= X .+ Y ;;
-  Y ::= X .- Y ;;
-  X ::= X .- Y
-  [[ fun st => st X = n /\ st Y = m]].
-
-Theorem swap_correct : forall m n,
-    dec_correct (swap_dec m n).
-(* FILL IN HERE using verify tactic *) Admitted.
-
-(* ----------------------------------------------------------------- *)
-(** *** Simple Conditionals *)
-Definition if_minus_plus_com :=
-  IFB X <=? Y
-  THEN Z ::= Y .- X
-  ELSE Y ::= X .+ Z
-  FI.
-
-Definition if_minus_plus_dec :=
-  [[ fun st => True ]]
-  IFB X <=? Y  THEN
-    Z ::= Y .- X
-  ELSE
-    Y ::= X .+ Z
-  FI
-  [[ fun st => st Y = st X + st Z ]].
-
-Theorem if_minus_plus_correct :
-  dec_correct if_minus_plus_dec.
-(* FILL IN HERE using verify tactic *) Admitted.
-
-Definition if_minus_dec :=
-  [[ fun st => True ]]
-  IFB X <=? Y THEN
-    Z ::= Y .- X
-  ELSE
-    Z ::= X .- Y
-  FI
-  [[ fun st => st Z + st X = st Y \/ st Z + st Y = st X ]].
-
-Theorem if_minus_correct :
-  dec_correct if_minus_dec.
-(* FILL IN HERE using verify tactic *) Admitted.
-
-(* ----------------------------------------------------------------- *)
-(** *** Division *)
-Definition div_mod_dec (a b : nat) : decorated :=
-  [[ fun st => True ]]
-  X ::= a ;;
-  Y ::= 0 ;;
-  WHILE b <=? X
-  [[ fun st => b * st Y + st X = a ]]
-  DO
-    X ::= X .- b ;;
-    Y ::= Y .+ 1
-  END
-  [[ fun st => b * st Y + st X = a /\ (st X < b) ]].
-
-Theorem div_mod_dec_correct : forall a b,
-  dec_correct (div_mod_dec a b).
-(* FILL IN HERE using verify tactic. HINT: mult_plus_distr_l *) Admitted.
-
-Local Opaque minus mult plus.
-
-(* ----------------------------------------------------------------- *)
-(** *** Square Roots *)
-Definition sqrt_dec m : decorated :=
-  [[ fun st => st X = m ]]
-  Z ::= 0 ;;
-  WHILE (Z .+ 1) .* (Z .+ 1) <=? X
-  [[ fun st => st X = m /\ st Z*st Z<=m ]]
-  DO
-    Z ::= Z .+ 1
-  END
-  [[ fun st => st Z*st Z<=m /\ m<(st Z+1)*(st Z+1) ]].
-
-Theorem sqrt_correct : forall m,
-  dec_correct (sqrt_dec m).
-(* FILL IN HERE using verify tactic *) Admitted.
-
-(* ----------------------------------------------------------------- *)
-(** *** Two loops *)
-Definition two_loops_dec (a b c : nat) : decorated :=
-  [[ fun st => True ]]
-  X ::= 0 ;;
-  Y ::= 0 ;;
-  Z ::= c ;;
-  WHILE !(X =? a)
-  [[ fun st => st Z = st X + c /\ st Y = 0 ]]
-  DO
-    X ::= X .+ 1 ;;
-    Z ::= Z .+ 1
-  END ;;
-  WHILE !(Y =? b)
-  [[ fun st => st Z = a + st Y + c ]]
-  DO
-    Y ::= Y .+ 1 ;;
-    Z ::= Z .+ 1
-  END
-  [[ fun st => st Z = a + b + c ]].
-
-Theorem two_loops_correct : forall a b c,
-  dec_correct (two_loops_dec a b c).
-(* FILL IN HERE using verify tactic *) Admitted.
+(* ################################################################# *)
+(** * Problem 6 *)
+(** Hint: refer to the deterministic for the original com taught in class **)
+Theorem ceval_deterministic: forall (c:com) st st1 st2 s1 s2,
+     c / st \\ s1 / st1  ->
+     c / st \\ s2 / st2 ->
+     st1 = st2 /\ s1 = s2.
+Proof.
+  (* FILL IN HERE *) Admitted.
